Refactoring access

Access.v
@@ -1,16 +1,20 @@
 From Coq Require Logic.ClassicalFacts.
+From Coq Require Import Arith.Arith.
+From Coq Require Import Lia.
 
 From Elo Require Import Util.
 From Elo Require Import Array.
 From Elo Require Import Core.
 
+(* A term accesses an address if it refers to the address directly or 
+indirectly. *)
 Inductive access (m : mem) : tm -> addr -> Prop :=
   | access_mem : forall ad ad' T,
     access m m[ad'] ad ->
-    access m <{ & ad' :: T }> ad
+    access m <{ &ad' :: T }> ad
 
   | access_ref : forall ad T,
-    access m <{ & ad :: T }> ad
+    access m <{ &ad :: T }> ad
 
   | access_new : forall T t ad,
     access m t ad ->
@@ -58,12 +62,6 @@ Proof.
   intros * Hacc ?. induction Hacc; eauto using access.
 Qed.
 
-Local Axiom excluded_middle : ClassicalFacts.excluded_middle.
-
-Lemma access_dec : forall m t ad,
-  (access m t ad) \/ (~ access m t ad).
-Proof. eauto using excluded_middle. Qed.
-
 Ltac inversion_access :=
   match goal with
   | H : access _ TM_Unit        _ |- _ => inversion H; clear H
@@ -79,11 +77,18 @@ Ltac inversion_access :=
   | H : access _ (TM_Spawn _)   _ |- _ => inversion H; clear H
   end.
 
-Definition well_behaved_access (m : mem) (t : tm) :=
-  forall ad, access m t ad -> ad < length m.
+(* ------------------------------------------------------------------------- *)
+(* access-dec                                                                *)
+(* ------------------------------------------------------------------------- *)
+
+Local Axiom excluded_middle : ClassicalFacts.excluded_middle.
+
+Lemma access_dec : forall m t ad,
+  (access m t ad) \/ (~ access m t ad).
+Proof. eauto using excluded_middle. Qed.
 
 (* ------------------------------------------------------------------------- *)
-(* not_access                                                                *)
+(* not-access                                                                *)
 (* ------------------------------------------------------------------------- *)
 
 Inductive not_access (m : mem) : tm -> addr -> Prop :=
@@ -136,15 +141,348 @@ Theorem not_access_iff : forall m t ad,
   ~ access m t ad <-> not_access m t ad.
 Proof.
   intros. split; intros H; destruct t;
-  try ( eapply not_access_ref
-       || eapply not_access_asg
-       || eapply not_access_call
-       || eapply not_access_seq);
+  try (eapply not_access_ref
+    || eapply not_access_asg
+    || eapply not_access_call
+    || eapply not_access_seq);
   eauto using access, not_access;
   intros ?; subst;
   try (inversion_access; inversion_clear H);
   eauto using access.
 Qed.
+
+(* ------------------------------------------------------------------------- *)
+(* valid-accesses                                                            *)
+(* ------------------------------------------------------------------------- *)
+
+Definition valid_accesses (m : mem) (t : tm) :=
+  forall ad, access m t ad -> ad < length m.
+
+(* ------------------------------------------------------------------------- *)
+(* va constructors                                                           *)
+(* ------------------------------------------------------------------------- *)
+
+Local Ltac solve_constructor_va := 
+  intros; intros ? ?; inversion_access; eauto.
+
+Local Lemma va_new: forall m t T,
+  valid_accesses m t ->
+  valid_accesses m <{ new T t }>.
+Proof. solve_constructor_va. Qed.
+
+Local Lemma va_load : forall m t,
+  valid_accesses m t ->
+  valid_accesses m <{ *t }>.
+Proof. solve_constructor_va. Qed.
+
+Local Lemma va_asg : forall m t1 t2,
+  valid_accesses m t1 ->
+  valid_accesses m t2 ->
+  valid_accesses m <{ t1 = t2 }>.
+Proof. solve_constructor_va. Qed.
+
+Local Lemma va_fun : forall m x Tx t,
+  valid_accesses m t ->
+  valid_accesses m <{ fn x Tx --> t }>.
+Proof. solve_constructor_va. Qed.
+
+Local Lemma va_call : forall m t1 t2,
+  valid_accesses m t1 ->
+  valid_accesses m t2 ->
+  valid_accesses m <{ call t1 t2 }>.
+Proof. solve_constructor_va. Qed.
+
+Local Lemma va_seq : forall m t1 t2,
+  valid_accesses m t1 ->
+  valid_accesses m t2 ->
+  valid_accesses m <{ t1; t2 }>.
+Proof. solve_constructor_va. Qed.
+
+(* ------------------------------------------------------------------------- *)
+(* inversion-valid-accesses                                                  *)
+(* ------------------------------------------------------------------------- *)
+
+Local Ltac solve_inversion_va := 
+  intros; unfold valid_accesses in *;
+  match goal with
+  | [ |- _ /\ _ ] => split
+  | [ |- _ ] => idtac
+  end;
+  eauto using access.
+
+Local Lemma inversion_va_ref : forall m ad T,
+  valid_accesses m <{ &ad :: T }> ->
+  valid_accesses m m[ad].
+Proof. solve_inversion_va. Qed.
+
+Local Lemma inversion_va_new : forall m t T,
+  valid_accesses m <{ new T t }> ->
+  valid_accesses m t.
+Proof. solve_inversion_va. Qed.
+
+Local Lemma inversion_va_load : forall m t,
+  valid_accesses m <{ *t }> ->
+  valid_accesses m t.
+Proof. solve_inversion_va. Qed.
+
+Local Lemma inversion_va_asg : forall m t1 t2,
+  valid_accesses m <{ t1 = t2 }> ->
+  valid_accesses m t1 /\ valid_accesses m t2.
+Proof. solve_inversion_va. Qed.
+
+Local Lemma inversion_va_fun : forall m x Tx t,
+  valid_accesses m <{ fn x Tx --> t }> ->
+  valid_accesses m t.
+Proof. solve_inversion_va. Qed.
+
+Local Lemma inversion_va_call : forall m t1 t2,
+  valid_accesses m <{ call t1 t2 }> ->
+  valid_accesses m t1 /\ valid_accesses m t2.
+Proof. solve_inversion_va. Qed.
+
+Local Lemma inversion_va_seq : forall m t1 t2,
+  valid_accesses m <{ t1; t2 }> ->
+  valid_accesses m t1 /\ valid_accesses m t2.
+Proof. solve_inversion_va. Qed.
+
+Ltac inversion_va :=
+  match goal with
+    | [ H : valid_accesses _ <{ &_ :: _ }>      |- _ ] =>
+        eapply inversion_va_ref in H as Hwba'
+    | [ H : valid_accesses _ <{ new _ _ }>      |- _ ] =>
+        eapply inversion_va_new in H
+    | [ H : valid_accesses _ <{ *_ }>           |- _ ] =>
+        eapply inversion_va_load in H
+    | [ H : valid_accesses _ <{ _ = _ }>        |- _ ] => 
+        eapply inversion_va_asg in H as [? ?]
+    | [ H : valid_accesses _ <{ fn _ _ --> _ }> |- _ ] => 
+        eapply inversion_va_fun in H
+    | [ H : valid_accesses _ <{ call _ _ }>     |- _ ] => 
+        eapply inversion_va_call in H as [? ?]
+    | [ H : valid_accesses _ <{ _; _ }>         |- _ ] => 
+        eapply inversion_va_seq in H as [? ?]
+  end.
+
+(* ------------------------------------------------------------------------- *)
+(* va -- value, mem & subst                                                  *)
+(* ------------------------------------------------------------------------- *)
+
+Local Lemma va_alloc_value : forall m t t' ad v,
+  valid_accesses m t ->
+  t --[EF_Alloc ad v]--> t' ->
+  valid_accesses m v.
+Proof.
+  intros. induction_step; inversion_va; eauto using access.
+Qed.
+
+Local Lemma va_write_value : forall m t t' ad v,
+  valid_accesses m t ->
+  t --[EF_Write ad v]--> t' ->
+  valid_accesses m v.
+Proof.
+  intros. induction_step; inversion_va; eauto using access.
+Qed.
+
+Ltac rewrite_array default :=
+  match goal with
+  (* get_add_eq *)
+  | H : context C [ (?l +++ _)[length ?l] ] |- _ =>
+    rewrite (get_add_eq default) in H; trivial
+  | |-  context C [ (?l +++ _)[length ?l] ] =>
+    rewrite (get_add_eq default); trivial
+  (* get_add_lt *)
+  | H : context C [ (?l +++ _)[?i] ], _ : ?i < length ?l |- _ => 
+    rewrite (get_add_lt default) in H; trivial
+  | _ : ?i < length ?l |- context C [ (?l +++ _)[?i] ] => 
+    rewrite (get_add_lt default); trivial
+  (* get_add_gt *)
+  | H : context C [ (?l +++ _)[?i] ], _ : length ?l < ?i |- _ => 
+    rewrite (get_add_gt default) in H; trivial
+  | _ : length ?l < ?i |- context C [ (?l +++ _)[?i] ] => 
+    rewrite (get_add_gt default); trivial
+  (* get_set_eq *)
+  | H : context C [ ?l[?i <- _ ][?i] ] |- _ =>
+    rewrite (get_set_eq default) in H; trivial
+  | |-  context C [ ?l[?i <- _ ][?i] ] =>
+    rewrite (get_set_eq default); trivial
+  (* get_set_neq *)
+  | H : context C [ ?l[?j <- _][?i] ], _ : ?i <> ?j |- _ => 
+    rewrite (get_set_neq default) in H; trivial
+  | H : context C [ ?l[?j <- _][?i] ], _ : ?j <> ?i |- _ => 
+    rewrite (get_set_neq default) in H; trivial
+  | _ : ?i <> ?j |- context C [ ?l[?j <- _][?i] ] => 
+    rewrite (get_set_neq default); trivial
+  | _ : ?j <> ?i |- context C [ ?l[?j <- _][?i] ] => 
+    rewrite (get_set_neq default); trivial
+  (* get_set_lt *)
+  | H : context C [ ?l[?j <- _][?i] ], _ : ?i < ?j |- _ => 
+    rewrite (get_set_lt default) in H; trivial
+  | _ : ?i < ?j |- context C [ ?l[?j <- _][?i] ] => 
+    rewrite (get_set_lt default); trivial
+  (* get_set_gt *)
+  | H : context C [ ?l[?j <- _][?i] ], _ : ?j < ?i |- _ => 
+    rewrite (get_set_gt default) in H; trivial
+  | _ : ?j < ?i |- context C [ ?l[?j <- _][?i] ] => 
+    rewrite (get_set_gt default); trivial
+  end.
+
+Local Lemma va_added_value : forall m v T,
+  valid_accesses (m +++ v) v ->
+  valid_accesses (m +++ v) <{ &(length m) :: T }>.
+Proof.
+  intros * ? ? Hacc.
+  remember (add m v) as m'.
+  remember (TM_Ref T (length m)) as t'.
+  induction Hacc; inversion Heqt'; subst.
+  - do 2 (rewrite_array TM_Unit). eauto using access.
+  - rewrite add_increments_length. lia.
+Qed.
+
+Local Lemma va_mem_add : forall m t v,
+  valid_accesses m t ->
+  valid_accesses (m +++ v) t.
+Proof.
+  intros * Hva ? Hacc. induction Hacc; subst; inversion_va; eauto.
+  - eapply IHHacc. intros ? ?.
+    destruct (lt_eq_lt_dec ad' (length m)) as [[? | ?] | ?]; subst;
+    do 3 (rewrite_array TM_Unit); eauto; try solve [inversion_access].
+    specialize (Hva (length m) (access_ref m (length m) _)). lia.
+  - rewrite add_increments_length. eauto using access, Nat.lt_lt_succ_r.
+Qed.
+
+Local Lemma va_mem_set : forall m t ad v,
+  valid_accesses m v ->
+  valid_accesses m t ->
+  valid_accesses m[ad <- v] t.
+Proof.
+  intros * ? ? ? Hacc.
+  rewrite set_preserves_length.
+  induction Hacc; inversion_va; eauto using access.
+  destruct (Nat.eq_dec ad ad'); subst;
+  do 2 (rewrite_array TM_Unit); eauto using access.
+Qed.
+
+Local Lemma va_subst : forall m t tx x,
+  valid_accesses m t ->
+  valid_accesses m tx ->
+  valid_accesses m ([x := tx] t).
+Proof.
+  intros. induction t;
+  try inversion_va; simpl; try (destruct String.string_dec);
+  eauto using va_new, va_load, va_asg, va_call, va_seq, va_fun.
+Qed.
+
+(* ------------------------------------------------------------------------- *)
+(* valid-accesses-preservation                                               *)
+(* ------------------------------------------------------------------------- *)
+
+Local Lemma va_none_preservation : forall m t t',
+  valid_accesses m t ->
+  t --[EF_None]--> t' ->
+  valid_accesses m t'.
+Proof.
+  intros. induction_step; inversion_va;
+  eauto using va_new, va_load, va_asg, va_fun, va_call, va_seq. 
+  inversion_va. eauto using va_subst.
+Qed.
+
+Local Lemma va_alloc_preservation : forall m t t' v,
+  valid_accesses m t ->
+  t --[EF_Alloc (length m) v]--> t' ->
+  valid_accesses (m +++ v) t'.
+Proof.
+  intros. induction_step; inversion_va;
+  eauto using va_new, va_load, va_asg, va_call, va_seq, va_mem_add,
+    va_added_value. 
+Qed.
+
+Local Lemma va_read_preservation : forall m t t' ad,
+  valid_accesses m t ->
+  t --[EF_Read ad m[ad]]--> t' ->
+  valid_accesses m t'.
+Proof.
+  intros. induction_step; inversion_va;
+  eauto using va_new, va_load, va_asg, va_call, va_seq.
+  intros ? ?. eauto using access.
+Qed.
+
+Local Lemma va_write_preservation : forall m t t' ad v,
+  valid_accesses m t ->
+  t --[EF_Write ad v]--> t' ->
+  valid_accesses m[ad <- v] t'.
+Proof.
+  intros.
+  assert (valid_accesses m v); eauto using va_write_value.
+  induction_step; inversion_va;
+  eauto using va_new, va_load, va_asg, va_call, va_seq, va_mem_set.
+  intros ? ?. inversion_access.
+Qed.
+
+Theorem va_mstep_preservation : forall m m' t t' eff,
+  valid_accesses m t ->
+  m / t ==[eff]==> m' / t' ->
+  valid_accesses m' t'.
+Proof.
+  intros. inversion_mstep;
+  eauto using va_none_preservation,
+    va_alloc_preservation,
+    va_read_preservation,
+    va_write_preservation.
+Qed.
+
+Definition va_memory (m : mem) := forall ad,
+  valid_accesses m m[ad].
+
+(* ------------------------------------------------------------------------- *)
+(* va memory                                                                 *)
+(* ------------------------------------------------------------------------- *)
+
+Local Lemma va_memory_alloc_preservation : forall m t t' v,
+  valid_accesses m t ->
+  (forall ad, valid_accesses m m[ad]) ->
+  t --[EF_Alloc (length m) v]--> t' ->
+  (forall ad, valid_accesses (m +++ v) (m +++ v)[ad]).
+Proof.
+  intros * Hva Hmva ? ad. induction_step; inversion_va; eauto.
+  decompose sum (lt_eq_lt_dec ad (length m)); subst;
+  rewrite_array TM_Unit; eauto using va_mem_add.
+  intros ? ?. inversion_access.
+Qed.
+
+Local Lemma va_memory_write_preservation : forall m t t' ad v,
+  valid_accesses m t ->
+  (forall ad, valid_accesses m m[ad]) ->
+  t --[EF_Write ad v]--> t' ->
+  (forall ad', valid_accesses m[ad <- v] m[ad <- v][ad']).
+Proof.
+  intros * Hva Hmva ? ad'. induction_step; inversion_va; eauto.
+  decompose sum (lt_eq_lt_dec ad ad'); subst;
+  rewrite_array TM_Unit; eauto using va_mem_set.
+  TODO
+Qed.
+
+Theorem memory_va_mstep_preservation : forall m m' t t' eff,
+  valid_accesses m t ->
+  va_memory m ->
+  m / t ==[eff]==> m' / t' ->
+  va_memory m'.
+Proof.
+  intros * Hva Hmva ?. inversion_mstep; trivial.
+  - induction_step; inversion_va; eauto.
+    intros ad.
+    decompose sum (lt_eq_lt_dec ad (length m)); subst; rewrite_array TM_Unit.
+    + eauto using va_mem_add.
+    + intros ad Hacc.
+      rewrite add_increments_length.
+      specialize (Hva ad).
+      eapply Nat.lt_lt_succ_r.
+      eapply Hva; clear Hva.
+      specialize (Hmva ad ad).
+    + 
+
+Qed.
+
+  forall ad ad', access m m[ad'] ad -> ad < length m.
 
 (* ------------------------------------------------------------------------- *)
 (* subst                                                                     *)
